Work on dummy adversary, simulator and dummy adversary theorem (just started). The MakeSimulator theory now changed to Simulator, and its theory parameters have changed. Dummy adversary theorem uses CombEnvAdv, which builds an environment out of the real environment and the adversary.
To facilitate connection with sequences of games involving MakeRF,
added to MakeRF

op adv_pis_rf_info_first (rfi : rf_info) : int
op adv_pis_rf_info_last (rfi : rf_info) : int

lemma adv_pis_rf_info_rangeset (rfi : rf_info) :
  adv_pis_rf_info rfi =
  rangeset (adv_pis_rf_info_first rfi) (adv_pis_rf_info_last rfi + 1).

lemma adv_pis_rf_info_first_ge1 (rfi : rf_info) :
  rf_info_valid rfi => 1 <= adv_pis_rf_info_first rfi.

lemma adv_pis_rf_info_first_le_last (rfi : rf_info) :
  rf_info_valid rfi =>
  adv_pis_rf_info_first rfi <= adv_pis_rf_info_last rfi.

common/UCCore.ec
@@ -201,8 +201,6 @@ by rewrite in_fsetU negb_or.
 by apply disj_ys_zs.
 qed.
 
-abstract theory MakeInterface.
-
 (* make interface out of functionality and adversary parts *)
 
 (* loop invariant for interface's while loop *)
@@ -243,6 +241,8 @@ op main_guard (func : addr, in_guard : int fset, m : msg) : bool =
   m.`1 = Adv /\ m.`2.`1 = adv /\
   (m.`2.`2 = 0 /\ m.`3 = env_root_port \/
    0 < m.`2.`2 /\ m.`2.`2 \in in_guard /\ envport func m.`3).
+
+abstract theory MakeInterface.
 
 module MI (Func : FUNC, Adv : ADV) : INTER = {
   var func : addr
@@ -700,6 +700,58 @@ conseq
 sim.
 qed.
 
+(* Converting Hoare lemmas about invariants and termination metrics
+   for adversaries into equiv lemmas
+
+   This will be used for simulator cores *)
+
+(* init lemma for use with any adversary, Adv, with an invariant
+   for which we know the corresponding hoare lemma *)
+
+lemma adv_init_invar_hoare_implies_equiv (Adv <: ADV)
+      (invar : glob Adv -> bool) :
+  hoare [Adv.init : true ==> invar (glob Adv)] =>
+  equiv
+  [Adv.init ~ Adv.init :
+   ={glob Adv} ==>
+   ={glob Adv} /\ invar (glob Adv){1}].
+proof.
+move => init_hoare.
+conseq
+  (_ : ={glob Adv} ==> ={glob Adv})
+  (_ : true ==> invar (glob Adv))
+  (_ : true ==> true) => //.
+sim.
+qed.
+
+(* invoke lemma for use with any adversary, Adv, with an invariant and
+   termination metric for which we know the corresponding hoare lemma *)
+
+lemma adv_invoke_term_metric_hoare_implies_equiv (Adv <: ADV)
+      (invar : glob Adv -> bool, tm : glob Adv -> int, n : int) :
+  hoare
+  [Adv.invoke :
+   invar (glob Adv) /\ tm (glob Adv) = n ==>
+   invar (glob Adv) /\
+   (res <> None => tm (glob Adv) < n)] =>
+  equiv
+  [Adv.invoke ~ Adv.invoke :
+   ={m, glob Adv} /\ invar (glob Adv){1} /\
+   tm (glob Adv){1} = n ==>
+   ={res, glob Adv} /\ invar (glob Adv){1} /\
+   (res{1} <> None => tm (glob Adv){1} < n)].
+proof.
+move => invoke_hoare.
+conseq
+  (_ : ={m, glob Adv} ==> ={glob Adv, res})
+  (_ :
+   invar (glob Adv) /\ tm (glob Adv) = n ==>
+   invar (glob Adv) /\
+   (res <> None => tm (glob Adv) < n))
+  (_ : true ==> true) => //.
+sim.
+qed.
+
 (* Wrapper for Real Functionalities
 
    Translator from UC DSL to EasyCrypt will turn real functionalities
@@ -728,6 +780,22 @@ op adv_pis_rf_info (rfi : rf_info) : int fset =
        (rfi.`rfi_adv_pi_main_end + 1)
   else rangeset rfi.`rfi_adv_pi_begin
        (nth1_adv_pi_end_params rfi rfi.`rfi_num_params + 1).
+
+op adv_pis_rf_info_first (rfi : rf_info) : int =
+  rfi.`rfi_adv_pi_begin.
+
+op adv_pis_rf_info_last (rfi : rf_info) : int =
+  if rfi.`rfi_num_params = 0
+  then rfi.`rfi_adv_pi_main_end
+  else nth1_adv_pi_end_params rfi rfi.`rfi_num_params.
+
+lemma adv_pis_rf_info_rangeset (rfi : rf_info) :
+  adv_pis_rf_info rfi =
+  rangeset (adv_pis_rf_info_first rfi) (adv_pis_rf_info_last rfi + 1).
+proof.
+rewrite /adv_pis_rf_info /adv_pis_rf_info_first /adv_pis_rf_info_last.
+by case (rfi.`rfi_num_params = 0).
+qed.
 
 op rf_info_valid (rfi : rf_info) : bool =
   1 <= rfi.`rfi_num_parties /\
@@ -797,6 +865,17 @@ have /# :
   ! (nth1_adv_pi_begin_params rfi 1 <= i <=
      nth1_adv_pi_end_params rfi j) by
     elim => [// | j ge0_j IH j_plus1_good_par /#].
+qed.
+
+lemma adv_pis_rf_info_first_ge1 (rfi : rf_info) :
+  rf_info_valid rfi => 1 <= adv_pis_rf_info_first rfi.
+proof. smt(). qed.
+
+lemma adv_pis_rf_info_first_le_last (rfi : rf_info) :
+  rf_info_valid rfi =>
+  adv_pis_rf_info_first rfi <= adv_pis_rf_info_last rfi.
+proof.
+smt(rfi_valid_adv_pi_main_end_lt_adv_pi_param_begin).
 qed.
 
 op addr_ge_param (rfi : rf_info, self addr : addr) : bool =
@@ -1165,16 +1244,13 @@ qed.
 
 end RealFunctionality.
 
-abstract theory DummyAdversary.
-
 (* dummy adversary (DA) - completely controlled by environment *)
 
 (* message from port env_root_port of environment to port
    adv_root_port (adv, 0) of dummy adversary, instructing dummy
    adversary to send message (Adv, dfe_pt, (adv, dfe_n), dfe_tag,
    dfe_u); this instruction will only be obeyed if 0 < dfe_n,
-   dfe_pt <> env_root_port, dfe_pt.`1 is not >= adv, and dfe_tag is
-   not TagNoInter *)
+   dfe_pt <> env_root_port and dfe_pt.`1 is not >= adv *)
 
 type da_from_env =
   {(* data: *)
@@ -1203,17 +1279,17 @@ op [opaque smt_opaque] dec_da_from_env (m : msg) : da_from_env option =
          in Some {|dfe_pt = pt; dfe_n = n; dfe_tag = tag; dfe_u = u|}
      end.
 
-op epdp_da_from_env_msg =
+op epdp_da_from_env =
   {|enc = enc_da_from_env; dec = dec_da_from_env|}.
 
-lemma valid_epdp_da_from_env_msg : valid_epdp epdp_da_from_env_msg.
+lemma valid_epdp_da_from_env : valid_epdp epdp_da_from_env.
 proof.
 apply epdp_intro.
 move => x.
-rewrite /epdp_da_from_env_msg /= /dec_da_from_env /enc_da_from_env /=.
+rewrite /epdp_da_from_env /= /dec_da_from_env /enc_da_from_env /=.
 by case x.
 move => [mod pt1 pt2 tag u] v.
-rewrite /epdp_da_from_env_msg /dec_da_from_env /enc_da_from_env /=.
+rewrite /epdp_da_from_env /dec_da_from_env /enc_da_from_env /=.
 case
   (mod = Dir \/ pt1 <> adv_root_port \/ pt2 <> env_root_port \/
    tag <> TagNoInter) => //.
@@ -1231,13 +1307,13 @@ rewrite val_u /= => <- /=.
 by rewrite (epdp_dec_enc _ _ u).
 qed.
 
-hint simplify [eqtrue] valid_epdp_da_from_env_msg.
-hint rewrite epdp : valid_epdp_da_from_env_msg.
+hint simplify [eqtrue] valid_epdp_da_from_env.
+hint rewrite epdp : valid_epdp_da_from_env.
 
 lemma eq_of_valid_da_from_env (m : msg) :
-  is_valid epdp_da_from_env_msg m =>
+  is_valid epdp_da_from_env m =>
   m =
-  let x = oget (epdp_da_from_env_msg.`dec m) in
+  let x = oget (epdp_da_from_env.`dec m) in
   (Adv,
    adv_root_port,
    env_root_port,
@@ -1247,10 +1323,10 @@ lemma eq_of_valid_da_from_env (m : msg) :
 proof.
 rewrite /is_valid.
 move => val_m.
-have [] x : exists (x : da_from_env), epdp_da_from_env_msg.`dec m = Some x.
-  exists (oget (epdp_da_from_env_msg.`dec m)); by rewrite -some_oget.
+have [] x : exists (x : da_from_env), epdp_da_from_env.`dec m = Some x.
+  exists (oget (epdp_da_from_env.`dec m)); by rewrite -some_oget.
 case x => x1 x2 x3 x4.
-move => /(epdp_dec_enc _ _ _ valid_epdp_da_from_env_msg) <- //.
+move => /(epdp_dec_enc _ _ _ valid_epdp_da_from_env) <- //.
 qed.
 
 (* message from port adv_root_port of dummy adversary to port
@@ -1288,17 +1364,17 @@ op [opaque smt_opaque] dec_da_to_env (m : msg) : da_to_env option =
         in Some {|dte_n = n; dte_pt = pt; dte_tag = tag; dte_u = u|}
      end.
 
-op epdp_da_to_env_msg =  (* let SMT provers inspect *)
+op epdp_da_to_env =  (* let SMT provers inspect *)
   {|enc = enc_da_to_env; dec = dec_da_to_env|}.
 
-lemma valid_epdp_da_to_env_msg : valid_epdp epdp_da_to_env_msg.
+lemma valid_epdp_da_to_env : valid_epdp epdp_da_to_env.
 proof.
 apply epdp_intro.
 move => x.
-rewrite /epdp_da_to_env_msg /= /dec_da_to_env /enc_da_to_env /=.
+rewrite /epdp_da_to_env /= /dec_da_to_env /enc_da_to_env /=.
 by case x.
 move => [mod pt1 pt2 tag u] v.
-rewrite /epdp_da_to_env_msg /dec_da_to_env /enc_da_to_env /=.
+rewrite /epdp_da_to_env /dec_da_to_env /enc_da_to_env /=.
 case (mod = Dir \/ pt1 <> env_root_port \/ pt2 <> adv_root_port \/
       tag <> TagNoInter) => //.
 rewrite !negb_or /= not_dir => [#] -> -> -> -> match_eq_some /=.
@@ -1315,13 +1391,13 @@ rewrite val_u /= => <- /=.
 by rewrite (epdp_dec_enc _ _ u).
 qed.
 
-hint simplify [eqtrue] valid_epdp_da_to_env_msg.
-hint rewrite epdp : valid_epdp_da_to_env_msg.
+hint simplify [eqtrue] valid_epdp_da_to_env.
+hint rewrite epdp : valid_epdp_da_to_env.
 
 lemma eq_of_valid_da_to_env (m : msg) :
-  is_valid epdp_da_to_env_msg m =>
+  is_valid epdp_da_to_env m =>
   m =
-  let x = oget (epdp_da_to_env_msg.`dec m) in
+  let x = oget (epdp_da_to_env.`dec m) in
   (Adv,
    env_root_port,
    adv_root_port,
@@ -1332,10 +1408,10 @@ lemma eq_of_valid_da_to_env (m : msg) :
 proof.
 rewrite /is_valid.
 move => val_m.
-have [] x : exists (x : da_to_env), epdp_da_to_env_msg.`dec m = Some x.
-  exists (oget (epdp_da_to_env_msg.`dec m)); by rewrite -some_oget.
+have [] x : exists (x : da_to_env), epdp_da_to_env.`dec m = Some x.
+  exists (oget (epdp_da_to_env.`dec m)); by rewrite -some_oget.
 case x => x1 x2 x3 x4.
-move => /(epdp_dec_enc _ _ _ valid_epdp_da_to_env_msg) <- //.
+move => /(epdp_dec_enc _ _ _ valid_epdp_da_to_env) <- //.
 qed.
 
 module DummyAdv : ADV = {
@@ -1344,10 +1420,11 @@ module DummyAdv : ADV = {
   proc invoke(m : msg) : msg option = {
     var r : msg option <- None;
 
-    match (epdp_da_from_env_msg.`dec m) with
+    match epdp_da_from_env.`dec m with
       Some x => {
+        (* m.`1 = Adv, m.`2 = adv_root_port, m.`3 = env_root_port *)
         if (0 < x.`dfe_n /\ x.`dfe_pt <> env_root_port /\
-            ! adv <= x.`dfe_pt.`1 /\ x.`dfe_tag <> TagNoInter) {
+            ! adv <= x.`dfe_pt.`1) {
           r <- Some (Adv, x.`dfe_pt, (adv, x.`dfe_n), x.`dfe_tag, x.`dfe_u);
         }
       }
@@ -1356,7 +1433,7 @@ module DummyAdv : ADV = {
            interface/simulator will enforce that m.`1 = Adv /\
            m.`2.`1 = adv /\ 0 <= m.`2.`2 /\ ! adv <= m.`3.`1 /\
            (m.`3 = env_root_port <=> m.`2.`2 = 0) *)
-        if (0 < m.`2.`2) {
+        if (0 < m.`2.`2) { (* so can't overlap with above *)
           r <-
             Some
             (enc_da_to_env
@@ -1369,8 +1446,6 @@ module DummyAdv : ADV = {
   }
 }.
 
-end DummyAdversary.
-
 (* module type for simulators
 
    a module that takes in Adv : ADV and yields an ADV will have this
@@ -1381,29 +1456,41 @@ module type SIM (Adv : ADV) = {
   proc invoke(m : msg) : msg option {Adv.invoke}
 }.
 
+(* simulator composition *)
+
 module (SimComp (Sim2 : SIM, Sim1 : SIM) : SIM) (Adv : ADV) : ADV =
   Sim2(Sim1(Adv)).
 
-abstract theory MakeSimulator.
+(* making simulators and dummy adversary theorem *)
 
-(* construct a simulator from a core *)
+abstract theory Simulator.
 
 (* begin theory parameters *)
 
-op core_pi : int.
+op adv_pis_begin : int.  (* first adversarial port index of unit *)
+op adv_pis_end   : int.  (* last adversarial port index of unit *)
 
-axiom core_pi_gt0 :
-  0 < core_pi.
+axiom adv_pis_begin_ge1    : 1 <= adv_pis_begin.
+axiom adv_pis_begin_le_end : adv_pis_begin <= adv_pis_end.
 
 (* end theory parameters *)
 
-(* loop invariant for simulator's while loop *)
+op sim_adv_pi : int      = adv_pis_begin.
+op adv_pis    : int fset = rangeset adv_pis_begin (adv_pis_end + 1).
+
+lemma sim_adv_pi_ge1 : 1 <= sim_adv_pi.
+proof.
+by rewrite /sim_adv_pi adv_pis_begin_ge1.
+qed.
+
+(* end theory parameters *)
 
 module (MS (Core : ADV) : SIM) (Adv : ADV) : ADV = {
   (* address of ideal functionality; only known after first message
-     received with destination port index core_pi *)
+     received with destination port index sim_adv_pi
 
-  (* if non-None, inc (oget if_addr_opt) adv *)
+     if non-None, inc (oget if_addr_opt) adv *)
+
   var if_addr_opt : addr option
 
   proc init() : unit = {
@@ -1424,7 +1511,7 @@ module (MS (Core : ADV) : SIM) (Adv : ADV) : ADV = {
         r <- None; not_done <- false;
       }
       elif (m.`2.`1 = adv) {
-        if (0 < m.`2.`2 /\ m.`2.`2 <> core_pi /\ if_addr <= m.`3.`1) {
+        if (0 < m.`2.`2 /\ m.`2.`2 <> sim_adv_pi /\ if_addr <= m.`3.`1) {
           not_done <- true;
         }
         else {
@@ -1432,7 +1519,7 @@ module (MS (Core : ADV) : SIM) (Adv : ADV) : ADV = {
         }
       }
       elif (m.`2.`1 = if_addr) {
-        if (m.`2.`2 = 1 /\ m.`3 = (adv, core_pi)) {
+        if (m.`2.`2 = 1 /\ m.`3 = (adv, sim_adv_pi)) {
           not_done <- false;
         }
         else {
@@ -1458,10 +1545,7 @@ module (MS (Core : ADV) : SIM) (Adv : ADV) : ADV = {
           ! (m.`3.`2 = 0 <=> m.`2 = env_root_port)) {
         r <- None; not_done <- false;
       }
-      elif (if_addr_opt = None) {
-        not_done <- false;
-      }
-      elif (oget if_addr_opt <= m.`2.`1) {
+      elif (if_addr_opt <> None /\ oget if_addr_opt <= m.`2.`1) {
         not_done <- true;
       }
       else {
@@ -1475,13 +1559,9 @@ module (MS (Core : ADV) : SIM) (Adv : ADV) : ADV = {
     var r : msg option <- None;
     var not_done : bool <- true;
 
-    (* not_done =>
-       (m.`2.`1 = adv \/
-        if_addr_opt <> None /\ oget if_addr_opt <= m.`2.`1) *)
-
     while (not_done) {
       if (m.`2.`1 = adv) {
-        if (m.`2.`2 = core_pi) {
+        if (m.`2.`2 = sim_adv_pi) {
           r <@ Core.invoke(m);
           (r, m, not_done) <@ after_core(r);
         }
@@ -1498,13 +1578,15 @@ module (MS (Core : ADV) : SIM) (Adv : ADV) : ADV = {
     return r;
   }
 
-  (* m.`1 = Adv /\ m.`2.`1 = adv /\
+  (* (if_addr_opt <> None => inc (oget if_addr_opt) adv) /\
+
+     m.`1 = Adv /\ m.`2.`1 = adv /\
      (m.`2.`2 = 0 /\ m.`3 = env_root_port \/
       0 < m.`2.`2 /\ ! adv <= m.`3.`1 /\ m.`3 <> env_root_port) *)
 
   proc invoke(m : msg) : msg option = {
     var r : msg option <- None;
-    if (m.`2.`2 = core_pi) {  (* so m.`3 <> env_root_port *)
+    if (m.`2.`2 = sim_adv_pi) {
       if (if_addr_opt = None) {
         if (m.`3.`2 = 1) {  (* ideal functionality's port index *)
           if_addr_opt <- Some m.`3.`1;
@@ -1522,4 +1604,420 @@ module (MS (Core : ADV) : SIM) (Adv : ADV) : ADV = {
   }
 }.
 
-end MakeSimulator.
+op after_core_return (if_addr : addr, r : msg option) : bool =
+  r <> None /\ (oget r).`1 = Adv /\ (oget r).`2.`1 = if_addr /\
+  (oget r).`2.`2 = 1 /\ (oget r).`3 = (adv, sim_adv_pi).
+
+op after_core_continue (if_addr : addr, r : msg option) : bool =
+  r <> None /\ (oget r).`1 = Adv /\ (oget r).`2.`1 = adv /\
+  0 < (oget r).`2.`2 /\ (oget r).`2.`2 <> sim_adv_pi /\
+  if_addr <= (oget r).`3.`1.
+
+op after_core_error (if_addr : addr, r : msg option) : bool =
+  r = None \/
+  (oget r).`1 = Dir \/
+  (oget r).`2.`1 = adv /\
+  (! 0 < (oget r).`2.`2 \/ ! (oget r).`2.`2 <> sim_adv_pi \/
+   ! if_addr <= (oget r).`3.`1) \/
+  (oget r).`2.`1 = if_addr /\
+  (! (oget r).`2.`2 = 1 \/ ! (oget r).`3 = (adv, sim_adv_pi)) \/
+  (oget r).`2.`1 <> adv /\ (oget r).`2.`1 <> if_addr.
+
+lemma after_core_disj (if_addr : addr, r : msg option) :
+  after_core_return if_addr r \/
+  after_core_continue if_addr r \/
+  after_core_error if_addr r.
+proof.
+smt().
+qed.
+
+lemma MS_after_core_return (CoreSim <: ADV) (Adv <: ADV)
+      (r' : msg option) :
+  phoare
+  [MS(CoreSim, Adv).after_core :
+   r = r' /\
+   MS.if_addr_opt <> None /\ inc (oget MS.if_addr_opt) adv /\
+   after_core_return (oget MS.if_addr_opt) r ==>
+   res.`1 = r' /\ res.`1 = Some res.`2 /\ ! res.`3] = 1%r.
+proof.
+proc; auto; smt(inc_ne_adv_func).
+qed.
+
+lemma MS_after_core_continue (CoreSim <: ADV) (Adv <: ADV)
+      (r' : msg option) :
+  phoare
+  [MS(CoreSim, Adv).after_core :
+   r = r' /\
+   after_core_continue (oget MS.if_addr_opt) r ==>
+   res.`1 = r' /\ res.`1 = Some res.`2 /\ res.`3] = 1%r.
+proof.
+proc; auto; smt().
+qed.
+
+lemma MS_after_core_error (CoreSim <: ADV) (Adv <: ADV)
+     (r' : msg option) :
+  phoare
+  [MS(CoreSim, Adv).after_core :
+   MS.if_addr_opt <> None /\ inc (oget MS.if_addr_opt) adv /\
+   after_core_error (oget MS.if_addr_opt) r ==>
+   res.`1 = None /\ ! res.`3] = 1%r.
+proof.
+proc; auto; smt(inc_ne_adv_func).
+qed.
+
+op after_adv_return (if_addr_opt : addr option, r : msg option) : bool =
+  r <> None /\ (oget r).`1 = Adv /\ ! adv <= (oget r).`2.`1 /\
+  (oget r).`3.`1 = adv /\ ! (oget r).`3.`2 < 0 /\
+  ((oget r).`3.`2 = 0 <=> (oget r).`2 = env_root_port) /\
+  (if_addr_opt = None \/ ! oget if_addr_opt <= (oget r).`2.`1).
+
+op after_adv_continue (if_addr_opt : addr option, r : msg option) : bool =
+  r <> None /\ (oget r).`1 = Adv /\ ! adv <= (oget r).`2.`1 /\
+  ! (oget r).`3.`1 <> adv /\ ! (oget r).`3.`2 < 0 /\
+  ((oget r).`3.`2 = 0 <=> (oget r).`2 = env_root_port) /\
+  (if_addr_opt <> None /\ oget if_addr_opt <= (oget r).`2.`1).
+
+op after_adv_error (if_addr_opt : addr option, r : msg option) : bool =
+  r = None \/ (oget r).`1 = Dir \/ adv <= (oget r).`2.`1 \/
+  (oget r).`3.`1 <> adv \/ (oget r).`3.`2 < 0 \/
+  ! ((oget r).`3.`2 = 0 <=> (oget r).`2 = env_root_port).
+
+lemma after_adv_disj (if_addr_opt : addr option, r : msg option) :
+  after_adv_return if_addr_opt r \/
+  after_adv_continue if_addr_opt r \/
+  after_adv_error if_addr_opt r.
+proof.
+smt().
+qed.
+
+lemma MS_after_adv_return (CoreSim <: ADV) (Adv <: ADV)
+      (r' : msg option) :
+  phoare
+  [MS(CoreSim, Adv).after_adv :
+   r = r' /\
+   after_adv_return MS.if_addr_opt r ==>
+   res.`1 = r' /\ res.`1 = Some res.`2 /\ ! res.`3] = 1%r.
+proof. proc; auto; smt(inc_ne_adv_func). qed.
+
+lemma MS_after_adv_continue (CoreSim <: ADV) (Adv <: ADV)
+      (r' : msg option) :
+  phoare
+  [MS(CoreSim, Adv).after_adv :
+   r = r' /\
+   after_adv_continue MS.if_addr_opt r ==>
+   res.`1 = r' /\ res.`1 = Some res.`2 /\ res.`3] = 1%r.
+proof. proc; auto; smt(). qed.
+
+lemma MS_after_adv_error (CoreSim <: ADV) (Adv <: ADV)
+     (r' : msg option) :
+  phoare
+  [MS(CoreSim, Adv).after_adv :
+   after_adv_error MS.if_addr_opt r ==>
+   res.`1 = None /\ ! res.`3] = 1%r.
+proof. proc; auto; smt(). qed.
+
+module (CombEnvAdv (Env : ENV, Adv : ADV) : ENV) (Inter : INTER) = {
+  var func : addr
+  var in_guard : int fset
+
+  module CombInter : INTER = {
+    proc init(func : addr, in_guard : int fset) : unit = { }
+
+    proc after_adv(r : msg option) : msg option * msg * bool * bool = {
+      var not_done : bool; var m : msg <- witness;
+      var adv_to_adv : bool <- witness;
+
+      if (r = None) {
+        not_done <- false;
+      }
+      else {
+        m <- oget r;
+        if (m.`1 = Dir \/ adv <= m.`2.`1 \/ adv <> m.`3.`1 \/ m.`3.`2 < 0) {
+          r <- None; not_done <- false;
+        }
+        elif (func <= m.`2.`1) {
+          if (m.`3.`2 = 0) {
+            r <- None; not_done <- false;
+          }
+          (* else: 0 < m.`3.`2 *)
+          m <-
+            epdp_da_from_env.`enc
+            {|dfe_pt = m.`2; dfe_n = m.`3.`2; dfe_tag = m.`4;
+              dfe_u = m.`5|};
+          r <- Some m; not_done <- true;
+          adv_to_adv <- false;  (* will be routed to Inter *)
+        }
+        else {  (* envport0 func m.`2 *)
+          not_done <- false;
+          if (! (m.`3.`2 = 0 <=> m.`2 = env_root_port)) {
+            r <- None;
+          }
+        }
+      }
+      return (r, m, not_done, adv_to_adv);
+    }
+
+    proc after_inter(r : msg option) : msg option * msg * bool * bool = {
+      var not_done : bool; var m : msg <- witness;
+      var adv_to_adv : bool <- witness; var dte : da_to_env;
+
+      if (r = None) {
+        not_done <- false;
+      }
+      else {
+        m <- oget r;
+        if (m.`1 = Dir) {
+          not_done <- false;
+        }
+        else {
+          dte <- oget (epdp_da_to_env.`dec m);
+          m <-
+            (Adv, (adv, dte.`dte_n), dte.`dte_pt,
+             dte.`dte_tag, dte.`dte_u);
+          r <- Some m; not_done <- true; adv_to_adv <- true;
+        }
+      }
+      return (r, m, not_done, adv_to_adv);
+    }
+
+    proc loop(m : msg) : msg option = {
+      var r : msg option <- None;
+      var not_done : bool <- true;
+
+      (* adversarial messages from environment will not go to dummy
+         adversary *)
+      var adv_to_adv : bool <- true;
+
+      while (not_done) {
+        if (m.`2.`1 = adv /\ adv_to_adv) {
+          r <@ Adv.invoke(m);
+          (r, m, not_done, adv_to_adv) <@ after_adv(r);
+        }
+        else {
+          r <@ Inter.invoke(m);
+          (r, m, not_done, adv_to_adv) <@ after_inter(r);
+        }
+      }
+      return r;
+    }
+
+    proc invoke(m : msg) : msg option = {
+      var r : msg option;
+      if (main_guard func in_guard m) {  (* usual guard for interface *)
+        r <@ loop(m);
+      }
+      else {
+        r <- None;
+      }
+      return r;
+    }
+  }
+
+  proc main(func_ : addr, in_guard_ : int fset) : bool = {
+    var b : bool;
+    func <- func_; in_guard <- in_guard_;
+    Adv.init();
+    b <@ Exper(CombInter, Env).main(func, in_guard);
+    return b;
+  }
+}.
+
+section.
+
+declare module Env       <: ENV{-MI, -CombEnvAdv}.
+declare module Adv       <: ADV{-MI, -CombEnvAdv, -Env}.
+declare module RealFunc  <: FUNC{-MI, -CombEnvAdv, -Env, -Adv}.
+declare module IdealFunc <: FUNC{-MI, -CombEnvAdv, -Env, -Adv}.
+declare module SimCore   <: ADV{-MI, -CombEnvAdv, -Env, -Adv, -IdealFunc}.
+
+declare op invar_rf : glob RealFunc -> bool.
+declare op term_rf  : glob RealFunc -> int.
+declare op invar_if : glob IdealFunc -> bool.
+declare op term_if  : glob IdealFunc -> int.
+declare op invar_sc : glob SimCore -> bool.
+declare op term_sc  : glob SimCore -> int.
+
+declare axiom ge0_term_rf (gl : glob RealFunc) :
+  invar_rf gl => 0 <= term_rf gl.
+
+declare axiom RealFunc_init :
+   equiv
+   [RealFunc.init ~ RealFunc.init :
+    ={self, glob RealFunc} ==>
+    ={glob RealFunc} /\ invar_rf (glob RealFunc){1}].
+
+declare axiom RealFunc_invoke (n : int) :
+   equiv
+   [RealFunc.invoke ~ RealFunc.invoke :
+    ={m, glob RealFunc} /\ invar_rf (glob RealFunc){1} /\
+    term_rf (glob RealFunc){1} = n ==>
+    ={res, glob RealFunc} /\ invar_rf (glob RealFunc){1} /\
+    (res{1} <> None =>
+     term_rf (glob RealFunc){1} < n /\
+     ((oget res{1}).`1 = Adv => (oget res{1}).`2.`2 \in adv_pis))].
+
+declare axiom ge0_term_if (gl : glob IdealFunc) :
+  invar_if gl => 0 <= term_if gl.
+
+declare axiom IdealFunc_init :
+   equiv
+   [IdealFunc.init ~ IdealFunc.init :
+    ={self, glob IdealFunc} ==>
+    ={glob IdealFunc} /\ invar_if (glob IdealFunc){1}].
+
+declare axiom IdealFunc_invoke (n : int) :
+   equiv
+   [IdealFunc.invoke ~ IdealFunc.invoke :
+    ={m, glob IdealFunc} /\ invar_if (glob IdealFunc){1} /\
+    term_if (glob IdealFunc){1} = n ==>
+    ={res, glob IdealFunc} /\ invar_if (glob IdealFunc){1} /\
+    (res{1} <> None =>
+     term_if (glob IdealFunc){1} < n /\
+     ((oget res{1}).`1 = Adv => (oget res{1}).`2.`2 \in adv_pis))].
+
+declare axiom ge0_term_sc (gl : glob SimCore) :
+  invar_sc gl => 0 <= term_sc gl.
+
+declare axiom SimCore_init :
+   equiv
+   [SimCore.init ~ SimCore.init :
+    ={glob SimCore} ==>
+    ={glob SimCore} /\ invar_sc (glob SimCore){1}].
+
+declare axiom SimCore_invoke (n : int) :
+   equiv
+   [SimCore.invoke ~ SimCore.invoke :
+    ={m, glob SimCore} /\ invar_sc (glob SimCore){1} /\
+    term_sc (glob SimCore){1} = n ==>
+    ={res, glob SimCore} /\ invar_sc (glob SimCore){1} /\
+    (res{1} <> None => term_sc (glob SimCore){1} < n)].
+
+local lemma bridge_real (func' : addr, in_guard' : int fset) &m :
+  Pr[Exper(MI(RealFunc, Adv), Env).main(func', in_guard') @ &m : res] =
+  Pr[Exper(MI(RealFunc, DummyAdv), CombEnvAdv(Env, Adv))
+       .main(func', in_guard') @ &m : res].
+proof.
+byequiv => //.
+proc.
+inline*.
+sp; wp.
+seq 2 10 :
+  (={glob RealFunc, glob Adv, glob Env} /\
+   func{1} = func' /\ in_guard{1} = in_guard' /\
+   func0{2} = func' /\ in_guard0{2} = in_guard' /\
+   MI.func{1} = func' /\ MI.in_guard{1} = in_guard' /\
+   MI.func{2} = func' /\ MI.in_guard{2} = in_guard' /\
+   CombEnvAdv.func{2} = func' /\ CombEnvAdv.in_guard{2} = in_guard').
+swap{2} 6 4; swap{2} 1 8.
+call (_ : true).
+call (_ : true).
+auto.
+call
+  (_ :
+   ={glob RealFunc, glob Adv} /\
+   MI.func{1} = func' /\ MI.in_guard{1} = in_guard' /\
+   MI.func{2} = func' /\ MI.in_guard{2} = in_guard' /\
+   CombEnvAdv.func{2} = func' /\ CombEnvAdv.in_guard{2} = in_guard').
+proc.
+if => //.
+inline{1} 1; inline{2} 1; sp 3 4.
+rcondt{1} 1; first auto. rcondt{2} 1; first auto.
+admit.
+auto.
+auto.
+qed.
+
+local lemma bridge_ideal (func' : addr, in_guard' : int fset) &m :
+  Pr[Exper(MI(IdealFunc, MS(SimCore, Adv)), Env)
+       .main(func', in_guard') @ &m : res] =
+  Pr[Exper(MI(IdealFunc, MS(SimCore, DummyAdv)), CombEnvAdv(Env, Adv))
+       .main(func', in_guard') @ &m : res].
+proof.
+admit.
+qed.
+
+lemma dummy_adv (func' : addr, in_guard' : int fset, b : real) &m :
+  exper_pre func' => disjoint in_guard' adv_pis =>
+  `|Pr[Exper(MI(RealFunc, DummyAdv), CombEnvAdv(Env, Adv))
+         .main(func', in_guard') @ &m : res] -
+    Pr[Exper(MI(IdealFunc, MS(SimCore, DummyAdv)), CombEnvAdv(Env, Adv))
+         .main(func', in_guard') @ &m : res]| <= b =>
+  `|Pr[Exper(MI(RealFunc, Adv), Env).main(func', in_guard') @ &m : res] -
+    Pr[Exper(MI(IdealFunc, MS(SimCore, Adv)), Env)
+         .main(func', in_guard') @ &m : res]| <= b.
+proof.
+move => ep_func' disj_ig' reduct.
+by rewrite bridge_real bridge_ideal.
+qed.
+
+end section.
+
+lemma dummy_adversary
+      (Env <: ENV{-MI, -CombEnvAdv}) (Adv <: ADV{-MI, -CombEnvAdv, -Env})
+      (RealFunc <: FUNC{-MI, -CombEnvAdv, -Env, -Adv})
+      (IdealFunc <: FUNC{-MI, -CombEnvAdv, -Env, -Adv})
+      (SimCore <: ADV{-MI, -CombEnvAdv, -Env, -Adv, -IdealFunc})
+      (invar_rf : glob RealFunc -> bool, term_rf : glob RealFunc -> int,
+       invar_if : glob IdealFunc -> bool, term_if : glob IdealFunc -> int,
+       invar_sc : glob SimCore -> bool, term_sc : glob SimCore -> int,
+       func' : addr, in_guard' : int fset, b : real) &m :
+  (forall (gl : glob RealFunc), invar_rf gl => 0 <= term_rf gl) =>
+  hoare [RealFunc.init : true ==> invar_rf (glob RealFunc)] =>
+  (forall (n : int),
+   hoare
+   [RealFunc.invoke :
+    invar_rf (glob RealFunc) /\ term_rf (glob RealFunc) = n ==>
+    invar_rf (glob RealFunc) /\
+    (res <> None =>
+       term_rf (glob RealFunc) < n /\
+       ((oget res).`1 = Adv => (oget res).`2.`2 \in adv_pis))]) =>
+  (forall (gl : glob IdealFunc), invar_if gl => 0 <= term_if gl) =>
+  hoare [IdealFunc.init : true ==> invar_if (glob IdealFunc)] =>
+  (forall (n : int),
+   hoare
+   [IdealFunc.invoke :
+    invar_if (glob IdealFunc) /\ term_if (glob IdealFunc) = n ==>
+    invar_if (glob IdealFunc) /\
+    (res <> None =>
+       term_if (glob IdealFunc) < n /\
+       ((oget res).`1 = Adv => (oget res).`2.`2 \in adv_pis))]) =>
+  (forall (gl : glob SimCore), invar_sc gl => 0 <= term_sc gl) =>
+  hoare [SimCore.init : true ==> invar_sc (glob SimCore)] =>
+  (forall (n : int),
+   hoare
+   [SimCore.invoke :
+    invar_sc (glob SimCore) /\ term_sc (glob SimCore) = n ==>
+    invar_sc (glob SimCore) /\
+    (res <> None => term_sc (glob SimCore) < n)]) =>
+  exper_pre func' => disjoint in_guard' adv_pis =>
+  `|Pr[Exper(MI(RealFunc, DummyAdv), CombEnvAdv(Env, Adv))
+         .main(func', in_guard') @ &m : res] -
+    Pr[Exper(MI(IdealFunc, MS(SimCore, DummyAdv)), CombEnvAdv(Env, Adv))
+         .main(func', in_guard') @ &m : res]| <= b =>
+  `|Pr[Exper(MI(RealFunc, Adv), Env).main(func', in_guard') @ &m : res] -
+    Pr[Exper(MI(IdealFunc, MS(SimCore, Adv)), Env)
+         .main(func', in_guard') @ &m : res]| <= b.
+proof.
+move =>
+  ge0_term_rf rf_init rf_invoke
+  ge0_term_if if_init if_invoke
+  ge0_term_sc sc_init sc_invoke
+  ep_func' disj_ig' reduct.
+apply
+  (dummy_adv
+   Env Adv RealFunc IdealFunc SimCore
+   invar_rf term_rf invar_if term_if invar_sc term_sc
+   ge0_term_rf _ _ ge0_term_if _ _ ge0_term_sc _ _
+   func' in_guard' b &m) => //.
+by apply (init_invar_hoare_implies_equiv RealFunc).
+move => n.
+rewrite (invoke_term_metric_hoare_implies_equiv RealFunc) rf_invoke.
+by apply (init_invar_hoare_implies_equiv IdealFunc).
+move => n.
+by rewrite (invoke_term_metric_hoare_implies_equiv IdealFunc) if_invoke.
+by apply (adv_init_invar_hoare_implies_equiv SimCore).
+move => n.
+rewrite (adv_invoke_term_metric_hoare_implies_equiv SimCore) sc_invoke.
+qed.
+
+end Simulator.
